add monitors

coq_alt/Lang.v
@@ -22,33 +22,6 @@ Section L.
   .
   Coercion Vnat : nat >-> value.
 
-  Inductive loc : Type :=
-  | addr : nat -> loc
-  .
-  Definition loc_eqb :=
-    fun ℓ1 ℓ2 =>
-      match ℓ1, ℓ2 with
-      | addr n1, addr n2 => Nat.eqb n1 n2
-      end
-  .
-  Lemma loc_eqb_eq ℓ0 ℓ1 :
-    loc_eqb ℓ0 ℓ1 = true <-> ℓ0 = ℓ1.
-  Proof.
-    destruct ℓ0 as [n0], ℓ1 as [n1]; split; intros H.
-    - cbn in H; rewrite Nat.eqb_eq in H; now subst.
-    - inv H; apply Nat.eqb_refl.
-  Qed.
-  #[export]
-  Instance loceq__Instance : HasEquality loc := {
-    eq := loc_eqb ;
-    eqb_eq := loc_eqb_eq ;
-  }.
-  #[local]
-  Existing Instance varteq__Instance.
-
-  #[local]
-  Hint Resolve eqb_eq String.eqb_refl : core.
-
 (** * Actual Syntax *)
 
 (** Final Result (without error) *)
