coq_alt/Mon.v
@@ -1,0 +1,224 @@
+Set Implicit Arguments.
+Require Import Strings.String CSC.Util CSC.Sets.
+
+(** * This file defines the various monitors from the paper. *)
+
+(** General structure of monitors. This time as module for namespacing. *)
+Module Type MonitorT.
+  Parameter AbsState : Type.
+  Parameter EmptyState : AbsState.
+  Parameter AbsEv : Type.
+  Parameter MonCheck : AbsState -> option AbsEv -> AbsState -> Prop.
+  Parameter string_of_absev : AbsEv -> string.
+End MonitorT.
+
+Module BaseMonitor (M : MonitorT).
+  #[export]
+  Instance MonInstance : LangParams := {
+    State := M.AbsState;
+    Ev := M.AbsEv;
+    step := M.MonCheck;
+    string_of_event := M.string_of_absev;
+    is_value := fun _ => True;
+  }.
+End BaseMonitor.
+
+(** Monitor Composition *)
+Module CompMonitor (M1 M2 : MonitorT) : MonitorT.
+  Definition AbsState : Type := (M1.AbsState * M2.AbsState).
+  Definition EmptyState : AbsState := (M1.EmptyState, M2.EmptyState).
+  Definition AbsEv : Type := (option M1.AbsEv * option M2.AbsEv).
+  Inductive MonCheck_i : AbsState -> option AbsEv -> AbsState -> Prop :=
+  | combinedCheck (T1 T1' : M1.AbsState) (T2 T2' : M2.AbsState)
+      (a1 : option M1.AbsEv) (a2 : option M2.AbsEv) :
+    M1.MonCheck T1 a1 T1' ->
+    M2.MonCheck T2 a2 T2' ->
+    MonCheck_i (T1, T2) (Some (a1, a2)) (T1', T2')
+  .
+  Definition MonCheck := MonCheck_i.
+  #[export]
+  Hint Unfold MonCheck : core.
+  Definition string_of_absev :=
+    fun a => let '(a1, a2) := a in
+          let s1 := match a1 with
+                    | Some x => M1.string_of_absev x
+                    | None => "ε"%string
+                    end in
+          let s2 := match a2 with
+                    | Some x => M2.string_of_absev x
+                    | None => "ε"%string
+                    end in
+          String.append "("%string (String.append s1
+                                      (String.append ";"%string
+                                         (String.append s2
+                                            ")"%string)))
+  .
+
+  #[export]
+  Instance MonInstance : LangParams := {
+    State := AbsState;
+    Ev := AbsEv;
+    step := MonCheck;
+    string_of_event := string_of_absev;
+    is_value := fun _ => True;
+  }.
+End CompMonitor.
+
+(** Temporal Memory Safety Monitor *)
+Module TMSMon : MonitorT.
+  Record AbsState_r : Type := {
+      alloced : Util.LocListSet ;
+      freed : Util.LocListSet ;
+    }.
+  Definition AbsState := AbsState_r.
+  #[export]
+  Hint Unfold AbsState : core.
+  Definition EmptyState : AbsState := {|
+    alloced := List.nil ;
+    freed := List.nil ;
+  |}.
+  Variant AbsEv_d : Type :=
+  | AAbort
+  | AAlloc (l : loc)
+  | AUse (l : loc)
+  | ADealloc (l : loc)
+  .
+  Definition AbsEv := AbsEv_d.
+  #[export]
+  Hint Unfold AbsEv : core.
+
+  Inductive MonCheck_i : AbsState -> option AbsEv -> AbsState -> Prop :=
+  | sms_uninteresting (T : AbsState) : MonCheck_i T None T
+  | sms_abort (T : AbsState) : MonCheck_i T (Some AAbort) EmptyState
+  | sms_use (T : AbsState) (l : loc) :
+    LocListSets.el l T.(alloced) ->
+    ~(LocListSets.el l T.(freed)) ->
+    MonCheck_i T (Some(AUse l)) T
+  | sms_alloc (T T' : AbsState) (l : loc) :
+    ~(LocListSets.el l T.(alloced)) ->
+    ~(LocListSets.el l T.(freed)) ->
+    T' = {|
+           alloced := LocListSets.Union T.(alloced) (List.cons l List.nil) ;
+           freed := T.(freed) ;
+         |} ->
+    MonCheck_i T (Some(AAlloc l)) T'
+  | sms_dealloc (T T' : AbsState) (l : loc) L0 L1 :
+    LocListSets.el l T.(alloced) ->
+    ~(LocListSets.el l T.(freed)) ->
+    T.(alloced) = List.app L0 (List.cons l L1) ->
+    T' = {|
+           alloced := List.app L0 L1 ;
+           freed := LocListSets.Union T.(freed) (List.cons l List.nil) ;
+         |} ->
+    MonCheck_i T (Some(AAlloc l)) T'
+  .
+  Definition MonCheck := MonCheck_i.
+  #[export]
+  Hint Unfold MonCheck : core.
+  Definition string_of_absev :=
+    fun a => match a with
+          | AAbort => "abs↯"%string
+          | AAlloc (addr _n) => "absAlloc ℓ"%string
+          | ADealloc (addr _n) => "absDealloc ℓ"%string
+          | AUse (addr _n) => "absUse ℓ"%string
+          end
+  .
+  #[export]
+  Instance MonInstance : LangParams := {
+    State := AbsState;
+    Ev := AbsEv;
+    step := MonCheck;
+    string_of_event := string_of_absev;
+    is_value := fun _ => True;
+  }.
+End TMSMon.
+
+(** Spatial Memory Safety Monitor *)
+Module LocNatList <: ListBase.
+  Definition A : Type := loc * nat.
+  Definition eqb := fun x y =>
+                      let '(l0, n0) := x in
+                      let '(l1, n1) := y in
+                      andb (loc_eqb l0 l1) (Nat.eqb n0 n1).
+End LocNatList.
+Module LocNatListSets <: Sig := SetTheoryList (LocNatList).
+Definition LocNatListSet := LocNatListSets.set.
+Module SMSMon : MonitorT.
+  Definition AbsState := LocNatListSet.
+  #[export]
+  Hint Unfold AbsState : core.
+  Definition EmptyState : AbsState := List.nil.
+  Variant AbsEv_d : Type :=
+  | AAbort
+  | AAlloc (l : loc) (n : nat)
+  | AUse (l : loc) (n : nat)
+  .
+  Definition AbsEv := AbsEv_d.
+  #[export]
+  Hint Unfold AbsEv : core.
+
+  Inductive MonCheck_i : AbsState -> option AbsEv -> AbsState -> Prop :=
+  | sms_uninteresting (T : AbsState) : MonCheck_i T None T
+  | sms_abort (T : AbsState) : MonCheck_i T (Some AAbort) EmptyState
+  | sms_use (T : AbsState) (l : loc) (n m : nat) :
+    LocNatListSets.el (l, m) T ->
+    n < m ->
+    MonCheck_i T (Some(AUse l n)) T
+  | sms_alloc (T T' : AbsState) (l : loc) (n : nat) :
+    (forall (m : nat), ~ LocNatListSets.el (l, m) T) ->
+    T' = LocNatListSets.Union T (List.cons (l,n) List.nil) ->
+    MonCheck_i T (Some(AAlloc l n)) T'
+  .
+  Definition MonCheck := MonCheck_i.
+  #[export]
+  Hint Unfold MonCheck : core.
+  Definition string_of_absev :=
+    fun a => match a with
+          | AAbort => "abs↯"%string
+          | AAlloc (addr _n) n => "absAlloc ℓ"%string
+          | AUse (addr _n) n => "absUse ℓ"%string
+          end
+  .
+  #[export]
+  Instance MonInstance : LangParams := {
+    State := AbsState;
+    Ev := AbsEv;
+    step := MonCheck;
+    string_of_event := string_of_absev;
+    is_value := fun _ => True;
+  }.
+End SMSMon.
+
+(** Strict Cryptographic Constan Time *)
+Module sCCTMon : MonitorT.
+  Definition AbsState : Type := unit.
+  Definition EmptyState : AbsState := tt.
+  Variant AbsEv_d : Type :=
+  | AAbort
+  | AAny
+  .
+  Definition AbsEv := AbsEv_d.
+  #[export]
+  Hint Unfold AbsEv : core.
+
+  Inductive MonCheck_i : AbsState -> option AbsEv -> AbsState -> Prop :=
+  | scct_abort (T : AbsState) : MonCheck_i T (Some AAbort) T
+  .
+  Definition MonCheck := MonCheck_i.
+  #[export]
+  Hint Unfold MonCheck : core.
+  Definition string_of_absev :=
+    fun a => match a with
+          | AAbort => "abs↯"%string
+          | AAny => "absAny"%string
+          end
+  .
+  #[export]
+  Instance MonInstance : LangParams := {
+    State := AbsState;
+    Ev := AbsEv;
+    step := MonCheck;
+    string_of_event := string_of_absev;
+    is_value := fun _ => True;
+  }.
+End sCCTMon.
